\documentclass{beamer}

\usepackage[utf8]{inputenc}
\usetheme{default}

\input{macro.tex}

\title{First-arrival traveltime tomography based on the adjoint-state method}

\AtBeginSubsection[]
 {
  \begin{frame}<beamer>{Outline}
   \tableofcontents[currentsection,currentsubsection]   
  \end{frame}
 }

\begin{document}
 
 \begin{frame}
  \titlepage
 \end{frame}

 \begin{frame}{Outline}
  \tableofcontents
 \end{frame}
 
 \section{Introduction}
 
 \subsection{Motivation}
 
 \begin{frame}{Motivation}
  
 \end{frame}

 \section{Theory}
 
 \begin{frame}{Gradient of the misfit function}
 
  \begin{itemize}
   \item Misfit function for a single-shot
   \begin{equation}
    J({c}) = \frac{1}{2}\int_{\partial\Omega}d\boldsymbol{r}|T({c},\boldsymbol{r}) - T_{obs}(\boldsymbol{r})|^2
   \end{equation}
   
   \item Gradient method
   \begin{equation}
    {c}_{n+1} = {c}_n - \alpha_n\nabla J({c}_n),
   \end{equation}
    where $\alpha$ is a positive scalar.
  \end{itemize}

 \end{frame}

 \begin{frame}{Gradient of the misfit function}
  
  \begin{itemize}
   \item Extended misfit function
   \begin{eqnarray}
    L({c},t,\lambda) = &&\frac{1}{2}\int_{\partial\Omega}d\boldsymbol{r}|t(\boldsymbol{r}) - T_{obs}(\boldsymbol{r})|^2 \nonumber \\
    - &&\frac{1}{2}\int_\Omega d\boldsymbol{x}\lambda(\boldsymbol{x})\bigg(|\nabla t(\boldsymbol{x})|^2 - \frac{1}{{c}(\boldsymbol{x})^2}\bigg)
   \end{eqnarray}

   \item for $t(\boldsymbol{x}) = T(\boldsymbol{x})$
   \begin{equation}
    L({c},T,\lambda) = J({c})
   \end{equation}
   
  \end{itemize}

  
 \end{frame}


\begin{frame}
	\begin{equation}
\frac{\partial L}{\partial c} = - \int_{\Omega} dx\frac{\lambda(\vc{x})}{c^3(\vc{x})} =  \frac{\partial J}{\partial c}
	\end{equation}
	\begin{equation}
	\frac{\partial L}{\partial \lambda} = 0
	\end{equation}
	\begin{equation}
	\ddt[L] = 0
	\end{equation}
	\begin{equation}
	\frac{\partial L}{\partial t} =\int_{\partial\Omega} d\boldsymbol{r}(t(\boldsymbol{r}) - T_{obs}(\boldsymbol{r})) -
	\int_{\Omega}d\vc{x}\lambda(\vc{x})\nabla  t(\vc{x}) \cdot \ddt[\nabla t]
	\end{equation}
	\begin{eqnarray}
		\frac{\partial L}{\partial t}& =  & \int_{\partial\Omega} d\boldsymbol{r}(t(\boldsymbol{r}) - T_{obs}(\boldsymbol{r}) - \lambda \vc{n} \cdot \nabla t) \nonumber \\
		&& + \int_{\Omega} d\vc{x}\nabla \cdot \lambda(\vc{x})\nabla T(\vc{x})
	\end{eqnarray}
	\begin{equation}
	\Delta(\vc{r})\vc{n}(\vc{r}) \cdot  \nabla T(\vc{r}) = T(\vc{r})  - T_{obs}(\vc{r})
	\end{equation}
	\begin{equation}
	\nabla \cdot \Delta(\vc{x})\nabla T(\vc{x}) = 0
	\end{equation}
	
	
\end{frame}

\end{document}
